thys/Transition_Systems_and_Automata/Automata/DBA/DGBA.thy
@@ -1,9 +1,7 @@
 section \<open>Deterministic Generalized Büchi Automata\<close>
 
 theory DGBA
-imports
-  "DBA"
-  "../../Basic/Degeneralization"
+imports "../Deterministic"
 begin
 
   datatype ('label, 'state) dgba = dgba
@@ -12,135 +10,16 @@ begin
     (transition: "'label \<Rightarrow> 'state \<Rightarrow> 'state")
     (accepting: "'state pred gen")
 
-  global_interpretation dgba: transition_system_initial
-    "transition A" "\<lambda> a p. a \<in> alphabet A" "\<lambda> p. p = initial A"
-    for A
-    defines path = dgba.path and run = dgba.run and reachable = dgba.reachable and nodes = dgba.nodes and
-      enableds = dgba.enableds and paths = dgba.paths and runs = dgba.runs
-    by this
+  global_interpretation dgba: automaton dgba alphabet initial transition accepting
+    defines path = dgba.path and run = dgba.run and reachable = dgba.reachable and nodes = dgba.nodes
+    by unfold_locales auto
+  global_interpretation dgba: automaton_trace dgba alphabet initial transition accepting "gen infs"
+    defines language = dgba.language
+    by standard
 
   abbreviation target where "target \<equiv> dgba.target"
   abbreviation states where "states \<equiv> dgba.states"
   abbreviation trace where "trace \<equiv> dgba.trace"
-
-  abbreviation successors :: "('label, 'state) dgba \<Rightarrow> 'state \<Rightarrow> 'state set" where
-    "successors \<equiv> dgba.successors TYPE('label)"
-
-  lemma path_alt_def: "path A w p \<longleftrightarrow> set w \<subseteq> alphabet A"
-  unfolding lists_iff_set[symmetric]
-  proof
-    show "w \<in> lists (alphabet A)" if "path A w p" using that by (induct arbitrary: p) (auto)
-    show "path A w p" if "w \<in> lists (alphabet A)" using that by (induct arbitrary: p) (auto)
-  qed
-  lemma run_alt_def: "run A w p \<longleftrightarrow> sset w \<subseteq> alphabet A"
-  unfolding streams_iff_sset[symmetric]
-  proof
-    show "w \<in> streams (alphabet A)" if "run A w p"
-      using that by (coinduction arbitrary: w p) (force elim: dgba.run.cases)
-    show "run A w p" if "w \<in> streams (alphabet A)"
-      using that by (coinduction arbitrary: w p) (force elim: streams.cases)
-  qed
-
-  definition language :: "('label, 'state) dgba \<Rightarrow> 'label stream set" where
-    "language A \<equiv> {w. run A w (initial A) \<and> gen infs (accepting A) (trace A w (initial A))}"
-
-  lemma language[intro]:
-    assumes "run A w (initial A)" "gen infs (accepting A) (trace A w (initial A))"
-    shows "w \<in> language A"
-    using assms unfolding language_def by auto
-  lemma language_elim[elim]:
-    assumes "w \<in> language A"
-    obtains "run A w (initial A)" "gen infs (accepting A) (trace A w (initial A))"
-    using assms unfolding language_def by auto
-
-  lemma language_alphabet: "language A \<subseteq> streams (alphabet A)"
-    unfolding language_def run_alt_def using sset_streams by auto
-
-  definition dgbad :: "('label, 'state) dgba \<Rightarrow> ('label, 'state degen) dba" where
-    "dgbad A \<equiv> dba
-      (alphabet A)
-      (initial A, 0)
-      (\<lambda> a (p, k). (transition A a p, count (accepting A) p k))
-      (degen (accepting A))"
-
-  lemma dgbad_simps[simp]:
-    "dba.alphabet (dgbad A) = alphabet A"
-    "dba.initial (dgbad A) = (initial A, 0)"
-    "dba.transition (dgbad A) a (p, k) = (transition A a p, count (accepting A) p k)"
-    "dba.accepting (dgbad A) = degen (accepting A)"
-    unfolding dgbad_def by auto
-
-  lemma dgbad_target[simp]: "dba.target (dgbad A) w (p, k) =
-    (dgba.target A w p, fold (count (accepting A)) (butlast (p # dgba.states A w p)) k)"
-    by (induct w arbitrary: p k) (auto)
-  lemma dgbad_states[simp]: "dba.states (dgbad A) w (p, k) =
-    dgba.states A w p || scan (count (accepting A)) (p # dgba.states A w p) k"
-    by (induct w arbitrary: p k) (auto)
-  lemma dgbad_trace[simp]: "dba.trace (dgbad A) w (p, k) =
-    dgba.trace A w p ||| sscan (count (accepting A)) (p ## dgba.trace A w p) k"
-    by (coinduction arbitrary: w p k) (auto)
-  lemma dgbad_path[iff]: "dba.path (dgbad A) w (p, k) \<longleftrightarrow> dgba.path A w p"
-    unfolding DBA.path_alt_def DGBA.path_alt_def by simp
-  lemma dgbad_run[iff]: "dba.run (dgbad A) w (p, k) \<longleftrightarrow> dgba.run A w p"
-    unfolding DBA.run_alt_def DGBA.run_alt_def by simp
-
-  (* TODO: revise *)
-  lemma dgbad_nodes_fst[simp]: "fst ` DBA.nodes (dgbad A) = DGBA.nodes A"
-    unfolding dba.nodes_alt_def dba.reachable_alt_def
-    unfolding dgba.nodes_alt_def dgba.reachable_alt_def
-    unfolding image_def by simp
-  lemma dgbad_nodes_snd_empty:
-    assumes "accepting A = []"
-    shows "snd ` DBA.nodes (dgbad A) \<subseteq> {0}"
-  proof -
-    have 2: "snd (dba.transition (dgbad A) a (p, k)) = 0" for a p k using assms by auto
-    show ?thesis using 2 by (auto elim: dba.nodes.cases)
-  qed
-  lemma dgbad_nodes_snd_nonempty:
-    assumes "accepting A \<noteq> []"
-    shows "snd ` DBA.nodes (dgbad A) \<subseteq> {0 ..< length (accepting A)}"
-  proof -
-    have 1: "snd (dba.initial (dgbad A)) < length (accepting A)"
-      using assms by simp
-    have 2: "snd (dba.transition (dgbad A) a (p, k)) < length (accepting A)" for a p k
-      using assms by auto
-    show ?thesis using 1 2 by (auto elim: dba.nodes.cases)
-  qed
-  lemma dgbad_nodes_empty:
-    assumes "accepting A = []"
-    shows "DBA.nodes (dgbad A) = DGBA.nodes A \<times> {0}"
-  proof -
-    have "(p, k) \<in> DBA.nodes (dgbad A) \<longleftrightarrow> p \<in> fst ` DBA.nodes (dgbad A) \<and> k = 0" for p k
-      using dgbad_nodes_snd_empty[OF assms] by (force simp del: dgbad_nodes_fst)
-    then show ?thesis by auto
-  qed
-  lemma dgbad_nodes_nonempty:
-    assumes "accepting A \<noteq> []"
-    shows "DBA.nodes (dgbad A) \<subseteq> DGBA.nodes A \<times> {0 ..< length (accepting A)}"
-    using subset_fst_snd dgbad_nodes_fst[of A] dgbad_nodes_snd_nonempty[OF assms] by blast
-  lemma dgbad_nodes: "DBA.nodes (dgbad A) \<subseteq> DGBA.nodes A \<times> {0 ..< max 1 (length (accepting A))}"
-    using dgbad_nodes_empty dgbad_nodes_nonempty by force
-
-  lemma dgbad_language[simp]: "DBA.language (dgbad A) = DGBA.language A" by force
-
-  lemma dgbad_nodes_finite[iff]: "finite (DBA.nodes (dgbad A)) \<longleftrightarrow> finite (DGBA.nodes A)"
-  proof
-    show "finite (DGBA.nodes A)" if "finite (DBA.nodes (dgbad A))"
-      using that by (auto simp flip: dgbad_nodes_fst)
-    show "finite (DBA.nodes (dgbad A))" if "finite (DGBA.nodes A)"
-      using dgbad_nodes that finite_subset by fastforce
-  qed
-  lemma dgbad_nodes_card: "card (DBA.nodes (dgbad A)) \<le> max 1 (length (accepting A)) * card (DGBA.nodes A)"
-  proof (cases "finite (DGBA.nodes A)")
-    case True
-    have "card (DBA.nodes (dgbad A)) \<le> card (DGBA.nodes A \<times> {0 ..< max 1 (length (accepting A))})"
-      using dgbad_nodes True by (blast intro: card_mono)
-    also have "\<dots> = max 1 (length (accepting A)) * card (DGBA.nodes A)" unfolding card_cartesian_product by simp
-    finally show ?thesis by this
-  next
-    case False
-    then have "card (DGBA.nodes A) = 0" "card (DBA.nodes (dgbad A)) = 0" by auto
-    then show ?thesis by simp
-  qed
+  abbreviation successors where "successors \<equiv> dgba.successors TYPE('label)"
 
 end
