thys/Transition_Systems_and_Automata/Automata/DCA/DCA_Combine.thy
@@ -1,298 +1,109 @@
 section \<open>Deterministic Co-Büchi Automata Combinations\<close>
 
 theory DCA_Combine
-imports "DCA" "DGCA"
+imports DCA DGCA
 begin
 
-  definition dcai :: "('label, 'state\<^sub>1) dca \<Rightarrow> ('label, 'state\<^sub>2) dca \<Rightarrow>
-    ('label, 'state\<^sub>1 \<times> 'state\<^sub>2) dca" where
-    "dcai A B \<equiv> dca
-      (dca.alphabet A \<inter> dca.alphabet B)
-      (dca.initial A, dca.initial B)
-      (\<lambda> a (p, q). (dca.transition A a p, dca.transition B a q))
-      (\<lambda> (p, q). dca.rejecting A p \<or> dca.rejecting B q)"
+  global_interpretation degeneralization: automaton_degeneralization_trace
+    dgca dgca.alphabet dgca.initial dgca.transition dgca.rejecting "cogen fins"
+    dca dca.alphabet dca.initial dca.transition dca.rejecting fins
+    defines degeneralize = degeneralization.degeneralize
+    by unfold_locales auto
 
-  lemma dcai_fst[iff]: "infs (P \<circ> fst) (dca.trace (dcai A B) w (p, q)) \<longleftrightarrow> infs P (dca.trace A w p)"
-  proof -
-    let ?t = "dca.trace (dcai A B) w (p, q)"
-    have "infs (P \<circ> fst) ?t \<longleftrightarrow> infs P (smap fst ?t)" by (simp add: comp_def)
-    also have "smap fst ?t = dca.trace A w p" unfolding dcai_def by (coinduction arbitrary: w p q) (auto)
-    finally show ?thesis by this
-  qed
-  lemma dcai_snd[iff]: "infs (P \<circ> snd) (dca.trace (dcai A B) w (p, q)) \<longleftrightarrow> infs P (dca.trace B w q)"
-  proof -
-    let ?t = "dca.trace (dcai A B) w (p, q)"
-    have "infs (P \<circ> snd) ?t \<longleftrightarrow> infs P (smap snd ?t)" by (simp add: comp_def)
-    also have "smap snd ?t = dca.trace B w q" unfolding dcai_def by (coinduction arbitrary: w p q) (auto)
-    finally show ?thesis by this
-  qed
-  lemma dcai_nodes_fst[intro]: "fst ` DCA.nodes (dcai A B) \<subseteq> DCA.nodes A"
-  proof (rule subsetI, erule imageE)
-    fix pq p
-    assume "pq \<in> DCA.nodes (dcai A B)" "p = fst pq"
-    then show "p \<in> DCA.nodes A" unfolding dcai_def by (induct arbitrary: p) (auto)
-  qed
-  lemma dcai_nodes_snd[intro]: "snd ` DCA.nodes (dcai A B) \<subseteq> DCA.nodes B"
-  proof (rule subsetI, erule imageE)
-    fix pq q
-    assume "pq \<in> DCA.nodes (dcai A B)" "q = snd pq"
-    then show "q \<in> DCA.nodes B" unfolding dcai_def by (induct arbitrary: q) (auto)
-  qed
+  lemmas degeneralize_language[simp] = degeneralization.degeneralize_language[folded DCA.language_def]
+  lemmas degeneralize_nodes_finite[iff] = degeneralization.degeneralize_nodes_finite[folded DCA.nodes_def]
+  lemmas degeneralize_nodes_card = degeneralization.degeneralize_nodes_card[folded DCA.nodes_def]
 
-  lemma dcai_nodes_finite[intro]:
+  global_interpretation intersection: automaton_intersection_trace
+    dca.dca dca.alphabet dca.initial dca.transition dca.rejecting fins
+    dca.dca dca.alphabet dca.initial dca.transition dca.rejecting fins
+    dca.dca dca.alphabet dca.initial dca.transition dca.rejecting fins
+    "\<lambda> c\<^sub>1 c\<^sub>2 pq. (c\<^sub>1 \<circ> fst) pq \<or> (c\<^sub>2 \<circ> snd) pq"
+    defines intersect = intersection.combine
+    by (unfold_locales) (simp del: comp_apply)
+
+  lemmas intersect_language = intersection.combine_language
+  lemmas intersect_nodes_finite = intersection.combine_nodes_finite
+  lemmas intersect_nodes_card = intersection.combine_nodes_card
+
+  global_interpretation union: automaton_union_trace
+    dca.dca dca.alphabet dca.initial dca.transition dca.rejecting fins
+    dca.dca dca.alphabet dca.initial dca.transition dca.rejecting fins
+    dgca.dgca dgca.alphabet dgca.initial dgca.transition dgca.rejecting "cogen fins"
+    "\<lambda> c\<^sub>1 c\<^sub>2. [c\<^sub>1 \<circ> fst, c\<^sub>2 \<circ> snd]"
+    defines union' = union.combine
+    by unfold_locales auto
+
+  lemmas union'_language[simp] = union.combine_language[folded DGCA.language_def]
+  lemmas union'_nodes_finite = union.combine_nodes_finite[folded DGCA.nodes_def]
+  lemmas union'_nodes_card = union.combine_nodes_card[folded DGCA.nodes_def]
+
+  global_interpretation intersection_list: automaton_intersection_list_trace
+    dca.dca dca.alphabet dca.initial dca.transition dca.rejecting fins
+    dca.dca dca.alphabet dca.initial dca.transition dca.rejecting fins
+    "\<lambda> cs pp. \<exists> k < length cs. (cs ! k) (pp ! k)"
+    defines intersect_list = intersection_list.combine
+    by (unfold_locales) (simp add: comp_def)
+
+  lemmas intersect_list_language = intersection_list.combine_language
+  lemmas intersect_list_nodes_finite = intersection_list.combine_nodes_finite
+  lemmas intersect_list_nodes_card = intersection_list.combine_nodes_card
+
+  global_interpretation union_list: automaton_union_list_trace
+    dca.dca dca.alphabet dca.initial dca.transition dca.rejecting fins
+    dgca.dgca dgca.alphabet dgca.initial dgca.transition dgca.rejecting "cogen fins"
+    "\<lambda> cs. map (\<lambda> k pp. (cs ! k) (pp ! k)) [0 ..< length cs]"
+    defines union_list' = union_list.combine
+    by (unfold_locales) (auto simp: cogen_def comp_def)
+
+  lemmas union_list'_language[simp] = union_list.combine_language[folded DGCA.language_def]
+  lemmas union_list'_nodes_finite = union_list.combine_nodes_finite[folded DGCA.nodes_def]
+  lemmas union_list'_nodes_card = union_list.combine_nodes_card[folded DGCA.nodes_def]
+
+  abbreviation union where "union A B \<equiv> degeneralize (union' A B)"
+
+  lemma union_language[simp]:
+    assumes "dca.alphabet A = dca.alphabet B"
+    shows "DCA.language (union A B) = DCA.language A \<union> DCA.language B"
+    using assms by simp
+  lemma union_nodes_finite:
     assumes "finite (DCA.nodes A)" "finite (DCA.nodes B)"
-    shows "finite (DCA.nodes (dcai A B))"
-  proof (rule finite_subset)
-    show "DCA.nodes (dcai A B) \<subseteq> DCA.nodes A \<times> DCA.nodes B"
-      using dcai_nodes_fst dcai_nodes_snd unfolding image_subset_iff by force
-    show "finite (DCA.nodes A \<times> DCA.nodes B)" using assms by simp
-  qed
-  lemma dcai_nodes_card[intro]:
+    shows "finite (DCA.nodes (union A B))"
+    using union'_nodes_finite assms by simp
+  lemma union_nodes_card:
     assumes "finite (DCA.nodes A)" "finite (DCA.nodes B)"
-    shows "card (DCA.nodes (dcai A B)) \<le> card (DCA.nodes A) * card (DCA.nodes B)"
+    shows "card (DCA.nodes (union A B)) \<le> 2 * card (DCA.nodes A) * card (DCA.nodes B)"
   proof -
-    have "card (DCA.nodes (dcai A B)) \<le> card (DCA.nodes A \<times> DCA.nodes B)"
-    proof (rule card_mono)
-      show "finite (DCA.nodes A \<times> DCA.nodes B)" using assms by simp
-      show "DCA.nodes (dcai A B) \<subseteq> DCA.nodes A \<times> DCA.nodes B"
-        using dcai_nodes_fst dcai_nodes_snd unfolding image_subset_iff by force
-    qed
-    also have "\<dots> = card (DCA.nodes A) * card (DCA.nodes B)" using card_cartesian_product by this
-    finally show ?thesis by this
-  qed
-
-  lemma dcai_language[simp]: "DCA.language (dcai A B) = DCA.language A \<inter> DCA.language B"
-  proof -
-    have 1: "dca.alphabet (dcai A B) = dca.alphabet A \<inter> dca.alphabet B" unfolding dcai_def by simp
-    have 2: "dca.initial (dcai A B) = (dca.initial A, dca.initial B)" unfolding dcai_def by simp
-    have 3: "dca.rejecting (dcai A B) = (\<lambda> pq. (dca.rejecting A \<circ> fst) pq \<or> (dca.rejecting B \<circ> snd) pq)"
-      unfolding dcai_def by auto
-    have 4: "infs (dca.rejecting (dcai A B)) (DCA.trace (dcai A B) w (p, q)) \<longleftrightarrow>
-      infs (dca.rejecting A) (DCA.trace A w p) \<or> infs (dca.rejecting B) (DCA.trace B w q)" for w p q
-      unfolding 3 by blast
-    show ?thesis unfolding DCA.language_def DCA.run_alt_def 1 2 4 by auto
-  qed
-
-  definition dcail :: "('label, 'state) dca list \<Rightarrow> ('label, 'state list) dca" where
-    "dcail AA \<equiv> dca
-      (\<Inter> (dca.alphabet ` set AA))
-      (map dca.initial AA)
-      (\<lambda> a pp. map2 (\<lambda> A p. dca.transition A a p) AA pp)
-      (\<lambda> pp. \<exists> k < length AA. dca.rejecting (AA ! k) (pp ! k))"
-
-  lemma dcail_trace_smap:
-    assumes "length pp = length AA" "k < length AA"
-    shows "smap (\<lambda> pp. pp ! k) (dca.trace (dcail AA) w pp) = dca.trace (AA ! k) w (pp ! k)"
-    using assms unfolding dcail_def by (coinduction arbitrary: w pp) (force)
-  lemma dcail_nodes_length:
-    assumes "pp \<in> DCA.nodes (dcail AA)"
-    shows "length pp = length AA"
-    using assms unfolding dcail_def by induct auto
-  lemma dcail_nodes[intro]:
-    assumes "pp \<in> DCA.nodes (dcail AA)" "k < length pp"
-    shows "pp ! k \<in> DCA.nodes (AA ! k)"
-    using assms unfolding dcail_def by induct auto
-
-  lemma dcail_finite[intro]:
-    assumes "list_all (finite \<circ> DCA.nodes) AA"
-    shows "finite (DCA.nodes (dcail AA))"
-  proof (rule finite_subset)
-    show "DCA.nodes (dcail AA) \<subseteq> listset (map DCA.nodes AA)"
-      by (force simp: listset_member list_all2_conv_all_nth dcail_nodes_length)
-    have "finite (listset (map DCA.nodes AA)) \<longleftrightarrow> list_all finite (map DCA.nodes AA)"
-      by (rule listset_finite) (auto simp: list_all_iff)
-    then show "finite (listset (map DCA.nodes AA))" using assms by (simp add: list.pred_map)
-  qed
-  lemma dcail_nodes_card:
-    assumes "list_all (finite \<circ> DCA.nodes) AA"
-    shows "card (DCA.nodes (dcail AA)) \<le> prod_list (map (card \<circ> DCA.nodes) AA)"
-  proof -
-    have "card (DCA.nodes (dcail AA)) \<le> card (listset (map DCA.nodes AA))"
-    proof (rule card_mono)
-      have "finite (listset (map DCA.nodes AA)) \<longleftrightarrow> list_all finite (map DCA.nodes AA)"
-        by (rule listset_finite) (auto simp: list_all_iff)
-      then show "finite (listset (map DCA.nodes AA))" using assms by (simp add: list.pred_map)
-      show "DCA.nodes (dcail AA) \<subseteq> listset (map DCA.nodes AA)"
-        by (force simp: listset_member list_all2_conv_all_nth dcail_nodes_length)
-    qed
-    also have "\<dots> = prod_list (map (card \<circ> DCA.nodes) AA)" by simp
-    finally show ?thesis by this
-  qed
-
-  lemma dcail_language[simp]: "DCA.language (dcail AA) = \<Inter> (DCA.language ` set AA)"
-  proof safe
-    fix A w
-    assume 1: "w \<in> DCA.language (dcail AA)" "A \<in> set AA"
-    obtain 2:
-      "dca.run (dcail AA) w (dca.initial (dcail AA))"
-      "fins (dca.rejecting (dcail AA)) (dca.trace (dcail AA) w (dca.initial (dcail AA)))"
-      using 1(1) by rule
-    obtain k where 3: "A = AA ! k" "k < length AA" using 1(2) unfolding in_set_conv_nth by auto
-    have 4: "fins (\<lambda> pp. dca.rejecting A (pp ! k)) (dca.trace (dcail AA) w (map dca.initial AA))"
-      using 2(2) 3 unfolding dcail_def by auto
-    show "w \<in> DCA.language A"
-    proof
-      show "dca.run A w (dca.initial A)"
-        using 1(2) 2(1) unfolding DCA.run_alt_def dcail_def by auto
-      have "True \<longleftrightarrow> fins (\<lambda> pp. dca.rejecting A (pp ! k)) (dca.trace (dcail AA) w (map dca.initial AA))"
-        using 4 by simp
-      also have "\<dots> \<longleftrightarrow> fins (dca.rejecting A) (smap (\<lambda> pp. pp ! k)
-        (dca.trace (dcail AA) w (map dca.initial AA)))" by (simp add: comp_def)
-      also have "smap (\<lambda> pp. pp ! k) (dca.trace (dcail AA) w (map dca.initial AA)) =
-        dca.trace (AA ! k) w (map dca.initial AA ! k)" using 3(2) by (fastforce intro: dcail_trace_smap)
-      also have "\<dots> = dca.trace A w (dca.initial A)" using 3 by auto
-      finally show "fins (dca.rejecting A) (DCA.trace A w (dca.initial A))" by simp
-    qed
-  next
-    fix w
-    assume 1: "w \<in> \<Inter> (DCA.language `set AA)"
-    have 2: "dca.run A w (dca.initial A)" "fins (dca.rejecting A) (dca.trace A w (dca.initial A))"
-      if "A \<in> set AA" for A using 1 that by auto
-    have 3: "fins (\<lambda> pp. dca.rejecting (AA ! k) (pp ! k)) (dca.trace (dcail AA) w (map dca.initial AA))"
-      if "k < length AA" for k
-    proof -
-      have "True \<longleftrightarrow> fins (dca.rejecting (AA ! k)) (dca.trace (AA ! k) w (map dca.initial AA ! k))"
-        using 2(2) that by auto
-      also have "dca.trace (AA ! k) w (map dca.initial AA ! k) =
-        smap (\<lambda> pp. pp ! k) (dca.trace (dcail AA) w (map dca.initial AA))"
-        using that by (fastforce intro: dcail_trace_smap[symmetric])
-      also have "infs (dca.rejecting (AA ! k)) \<dots> \<longleftrightarrow> infs (\<lambda> pp. dca.rejecting (AA ! k) (pp ! k))
-        (dca.trace (dcail AA) w (map dca.initial AA))" by (simp add: comp_def)
-      finally show ?thesis by simp
-    qed
-    show "w \<in> DCA.language (dcail AA)"
-    proof
-      show "dca.run (dcail AA) w (dca.initial (dcail AA))"
-        using 2(1) unfolding DCA.run_alt_def dcail_def by auto
-      show "fins (dca.rejecting (dcail AA)) (dca.trace (dcail AA) w (dca.initial (dcail AA)))"
-        using 3 unfolding dcail_def by auto
-    qed
-  qed
-
-  definition dcgaul :: "('label, 'state) dca list \<Rightarrow> ('label, 'state list) dgca" where
-    "dcgaul AA \<equiv> dgca
-      (\<Union> (dca.alphabet ` set AA))
-      (map dca.initial AA)
-      (\<lambda> a pp. map2 (\<lambda> A p. dca.transition A a p) AA pp)
-      (map (\<lambda> k pp. dca.rejecting (AA ! k) (pp ! k)) [0 ..< length AA])"
-
-  lemma dcgaul_trace_smap:
-    assumes "length pp = length AA" "k < length AA"
-    shows "smap (\<lambda> pp. pp ! k) (dgca.trace (dcgaul AA) w pp) = dca.trace (AA ! k) w (pp ! k)"
-    using assms unfolding dcgaul_def by (coinduction arbitrary: w pp) (force)
-  lemma dcgaul_nodes_length:
-    assumes "pp \<in> DGCA.nodes (dcgaul AA)"
-    shows "length pp = length AA"
-    using assms unfolding dcgaul_def by induct auto
-  lemma dcgaul_nodes[intro]:
-    assumes "\<Inter> (dca.alphabet ` set AA)  = \<Union> (dca.alphabet ` set AA)"
-    assumes "pp \<in> DGCA.nodes (dcgaul AA)" "k < length pp"
-    shows "pp ! k \<in> DCA.nodes (AA ! k)"
-    using assms(2, 3, 1) unfolding dcgaul_def by induct force+
-
-  lemma dcgaul_nodes_finite[intro]:
-    assumes "\<Inter> (dca.alphabet ` set AA)  = \<Union> (dca.alphabet ` set AA)"
-    assumes "list_all (finite \<circ> DCA.nodes) AA"
-    shows "finite (DGCA.nodes (dcgaul AA))"
-  proof (rule finite_subset)
-    show "DGCA.nodes (dcgaul AA) \<subseteq> listset (map DCA.nodes AA)"
-      using assms(1) by (force simp: listset_member list_all2_conv_all_nth dcgaul_nodes_length)
-    have "finite (listset (map DCA.nodes AA)) \<longleftrightarrow> list_all finite (map DCA.nodes AA)"
-      by (rule listset_finite) (auto simp: list_all_iff)
-    then show "finite (listset (map DCA.nodes AA))" using assms(2) by (simp add: list.pred_map)
-  qed
-  lemma dcgaul_nodes_card:
-    assumes "\<Inter> (dca.alphabet ` set AA)  = \<Union> (dca.alphabet ` set AA)"
-    assumes "list_all (finite \<circ> DCA.nodes) AA"
-    shows "card (DGCA.nodes (dcgaul AA)) \<le> prod_list (map (card \<circ> DCA.nodes) AA)"
-  proof -
-    have "card (DGCA.nodes (dcgaul AA)) \<le> card (listset (map DCA.nodes AA))"
-    proof (rule card_mono)
-      have "finite (listset (map DCA.nodes AA)) \<longleftrightarrow> list_all finite (map DCA.nodes AA)"
-        by (rule listset_finite) (auto simp: list_all_iff)
-      then show "finite (listset (map DCA.nodes AA))" using assms(2) by (simp add: list.pred_map)
-      show "DGCA.nodes (dcgaul AA) \<subseteq> listset (map DCA.nodes AA)"
-        using assms(1) by (force simp: listset_member list_all2_conv_all_nth dcgaul_nodes_length)
-    qed
-    also have "\<dots> = prod_list (map (card \<circ> DCA.nodes) AA)" by simp
-    finally show ?thesis by this
-  qed
-
-  lemma dcgaul_language[simp]:
-    assumes "\<Inter> (dca.alphabet ` set AA)  = \<Union> (dca.alphabet ` set AA)"
-    shows "DGCA.language (dcgaul AA) = \<Union> (DCA.language ` set AA)"
-  proof safe
-    fix w
-    assume 1: "w \<in> DGCA.language (dcgaul AA)"
-    obtain k where 2:
-      "dgca.run (dcgaul AA) w (dgca.initial (dcgaul AA))"
-      "k < length AA"
-      "fins (\<lambda> pp. dca.rejecting (AA ! k) (pp ! k)) (dgca.trace (dcgaul AA) w (dgca.initial (dcgaul AA)))"
-      using 1 unfolding dcgaul_def by force
-    show "w \<in> \<Union> (DCA.language ` set AA)"
-    proof (intro UN_I DCA.language)
-      show "AA ! k \<in> set AA" using 2(2) by simp
-      show "dca.run (AA ! k) w (dca.initial (AA ! k))"
-        using assms 2(1, 2) unfolding DCA.run_alt_def DGCA.run_alt_def dcgaul_def by force
-      have "True \<longleftrightarrow> fins (\<lambda> pp. dca.rejecting (AA ! k) (pp ! k))
-        (dgca.trace (dcgaul AA) w (map dca.initial AA))" using 2(3) unfolding dcgaul_def by auto
-      also have "\<dots> \<longleftrightarrow> fins (dca.rejecting (AA ! k))
-        (smap (\<lambda> pp. pp ! k) (dgca.trace (dcgaul AA) w (map dca.initial AA)))" by (simp add: comp_def)
-      also have "smap (\<lambda> pp. pp ! k) (dgca.trace (dcgaul AA) w (map dca.initial AA)) =
-        dca.trace (AA ! k) w (map dca.initial AA ! k)" using 2(2) by (fastforce intro: dcgaul_trace_smap)
-      also have "\<dots> = dca.trace (AA ! k) w (dca.initial (AA ! k))" using 2(2) by auto
-      finally show "fins (dca.rejecting (AA ! k)) (dca.trace (AA ! k) w (dca.initial (AA ! k)))" by simp
-    qed
-  next
-    fix A w
-    assume 1: "A \<in> set AA" "w \<in> DCA.language A"
-    obtain 2: "dca.run A w (dca.initial A)" "fins (dca.rejecting A) (dca.trace A w (dca.initial A))"
-      using 1(2) by rule
-    obtain k where 3: "A = AA ! k" "k < length AA" using 1(1) unfolding in_set_conv_nth by auto
-    show "w \<in> DGCA.language (dcgaul AA)"
-    proof (intro DGCA.language bexI cogen)
-      show "dgca.run (dcgaul AA) w (dgca.initial (dcgaul AA))"
-        using 1(1) 2(1) unfolding DCA.run_alt_def DGCA.run_alt_def dcgaul_def by auto
-      have "True \<longleftrightarrow> fins (dca.rejecting (AA ! k)) (dca.trace (AA ! k) w (map dca.initial AA ! k))"
-        using 2(2) 3 by auto
-      also have "dca.trace (AA ! k) w (map dca.initial AA ! k) =
-        smap (\<lambda> pp. pp ! k) (dgca.trace (dcgaul AA) w (map dca.initial AA))"
-        using 3(2) by (fastforce intro: dcgaul_trace_smap[symmetric])
-      also have "fins (dca.rejecting (AA ! k)) \<dots> \<longleftrightarrow> fins (\<lambda> pp. dca.rejecting (AA ! k) (pp ! k))
-        (dgca.trace (dcgaul AA) w (map dca.initial AA))" by (simp add: comp_def)
-      also have "map dca.initial AA = dgca.initial (dcgaul AA)" unfolding dcgaul_def by simp
-      finally show "fins (\<lambda> pp. dca.rejecting (AA ! k) (pp ! k)) (dgca.trace (dcgaul AA) w (dgca.initial (dcgaul AA)))"
-        by simp
-      show "(\<lambda> pp. dca.rejecting (AA ! k) (pp ! k)) \<in> set (dgca.rejecting (dcgaul AA))"
-        unfolding dcgaul_def using 3(2) by simp
-    qed
-  qed
-
-  definition dcaul :: "('label, 'state) dca list \<Rightarrow> ('label, 'state list degen) dca" where
-    "dcaul = dgcad \<circ> dcgaul"
-
-  lemma dcaul_nodes_finite[intro]:
-    assumes "\<Inter> (dca.alphabet ` set AA)  = \<Union> (dca.alphabet ` set AA)"
-    assumes "list_all (finite \<circ> DCA.nodes) AA"
-    shows "finite (DCA.nodes (dcaul AA))"
-    using dcgaul_nodes_finite assms unfolding dcaul_def by auto
-  lemma dcaul_nodes_card:
-    assumes "\<Inter> (dca.alphabet ` set AA)  = \<Union> (dca.alphabet ` set AA)"
-    assumes "list_all (finite \<circ> DCA.nodes) AA"
-    shows "card (DCA.nodes (dcaul AA)) \<le> max 1 (length AA) * prod_list (map (card \<circ> DCA.nodes) AA)"
-  proof -
-    have "card (DCA.nodes (dcaul AA)) \<le>
-      max 1 (length (dgca.rejecting (dcgaul AA))) * card (DGCA.nodes (dcgaul AA))"
-      unfolding dcaul_def using dgcad_nodes_card by simp
-    also have "length (dgca.rejecting (dcgaul AA)) = length AA" unfolding dcgaul_def by simp
-    also have "card (DGCA.nodes (dcgaul AA)) \<le> prod_list (map (card \<circ> DCA.nodes) AA)"
-      using dcgaul_nodes_card assms by this
+    have "card (DCA.nodes (union A B)) \<le>
+      max 1 (length (dgca.rejecting (union' A B))) * card (DGCA.nodes (union' A B))"
+      using degeneralize_nodes_card by this
+    also have "length (dgca.rejecting (union' A B)) = 2" by simp
+    also have "card (DGCA.nodes (union' A B)) \<le> card (DCA.nodes A) * card (DCA.nodes B)"
+      using union'_nodes_card assms by this
     finally show ?thesis by simp
   qed
 
-  lemma dcaul_language[simp]:
+  abbreviation union_list where "union_list AA \<equiv> degeneralize (union_list' AA)"
+
+  lemma union_list_language[simp]:
     assumes "\<Inter> (dca.alphabet ` set AA) = \<Union> (dca.alphabet ` set AA)"
-    shows "DCA.language (dcaul AA) = \<Union> (DCA.language ` set AA)"
-    unfolding dcaul_def using dgcad_language dcgaul_language[OF assms] by auto
+    shows "DCA.language (union_list AA) = \<Union> (DCA.language ` set AA)"
+    using assms by simp
+  lemma union_list_nodes_finite:
+    assumes "list_all (finite \<circ> DCA.nodes) AA"
+    shows "finite (DCA.nodes (union_list AA))"
+    using union_list'_nodes_finite assms by simp
+  lemma union_list_nodes_card:
+    assumes "list_all (finite \<circ> DCA.nodes) AA"
+    shows "card (DCA.nodes (union_list AA)) \<le> max 1 (length AA) * prod_list (map (card \<circ> DCA.nodes) AA)"
+  proof -
+    have "card (DCA.nodes (union_list AA)) \<le>
+      max 1 (length (dgca.rejecting (union_list' AA))) * card (DGCA.nodes (union_list' AA))"
+      using degeneralize_nodes_card by this
+    also have "length (dgca.rejecting (union_list' AA)) = length AA" by simp
+    also have "card (DGCA.nodes (union_list' AA)) \<le> prod_list (map (card \<circ> DCA.nodes) AA)"
+      using union_list'_nodes_card assms by this
+    finally show ?thesis by simp
+  qed
 
 end
