thys/Transition_Systems_and_Automata/Automata/DCA/DGCA.thy
@@ -1,9 +1,7 @@
 section \<open>Deterministic Co-Generalized Co-Büchi Automata\<close>
 
 theory DGCA
-imports
-  "DCA"
-  "../../Basic/Degeneralization"
+imports "../Deterministic"
 begin
 
   datatype ('label, 'state) dgca = dgca
@@ -12,135 +10,16 @@ begin
     (transition: "'label \<Rightarrow> 'state \<Rightarrow> 'state")
     (rejecting: "'state pred gen")
 
-  global_interpretation dgca: transition_system_initial
-    "transition A" "\<lambda> a p. a \<in> alphabet A" "\<lambda> p. p = initial A"
-    for A
-    defines path = dgca.path and run = dgca.run and reachable = dgca.reachable and nodes = dgca.nodes and
-      enableds = dgca.enableds and paths = dgca.paths and runs = dgca.runs
-    by this
+  global_interpretation dgca: automaton dgca alphabet initial transition rejecting
+    defines path = dgca.path and run = dgca.run and reachable = dgca.reachable and nodes = dgca.nodes
+    by unfold_locales auto
+  global_interpretation dgca: automaton_trace dgca alphabet initial transition rejecting "cogen fins"
+    defines language = dgca.language
+    by standard
 
   abbreviation target where "target \<equiv> dgca.target"
   abbreviation states where "states \<equiv> dgca.states"
   abbreviation trace where "trace \<equiv> dgca.trace"
-
-  abbreviation successors :: "('label, 'state) dgca \<Rightarrow> 'state \<Rightarrow> 'state set" where
-    "successors \<equiv> dgca.successors TYPE('label)"
-
-  lemma path_alt_def: "path A w p \<longleftrightarrow> set w \<subseteq> alphabet A"
-  unfolding lists_iff_set[symmetric]
-  proof
-    show "w \<in> lists (alphabet A)" if "path A w p" using that by (induct arbitrary: p) (auto)
-    show "path A w p" if "w \<in> lists (alphabet A)" using that by (induct arbitrary: p) (auto)
-  qed
-  lemma run_alt_def: "run A w p \<longleftrightarrow> sset w \<subseteq> alphabet A"
-  unfolding streams_iff_sset[symmetric]
-  proof
-    show "w \<in> streams (alphabet A)" if "run A w p"
-      using that by (coinduction arbitrary: w p) (force elim: dgca.run.cases)
-    show "run A w p" if "w \<in> streams (alphabet A)"
-      using that by (coinduction arbitrary: w p) (force elim: streams.cases)
-  qed
-
-  definition language :: "('label, 'state) dgca \<Rightarrow> 'label stream set" where
-    "language A \<equiv> {w. run A w (initial A) \<and> cogen fins (rejecting A) (trace A w (initial A))}"
-
-  lemma language[intro]:
-    assumes "run A w (initial A)" "cogen fins (rejecting A) (trace A w (initial A))"
-    shows "w \<in> language A"
-    using assms unfolding language_def by auto
-  lemma language_elim[elim]:
-    assumes "w \<in> language A"
-    obtains "run A w (initial A)" "cogen fins (rejecting A) (trace A w (initial A))"
-    using assms unfolding language_def by auto
-
-  lemma language_alphabet: "language A \<subseteq> streams (alphabet A)"
-    unfolding language_def run_alt_def using sset_streams by auto
-
-  definition dgcad :: "('label, 'state) dgca \<Rightarrow> ('label, 'state degen) dca" where
-    "dgcad A \<equiv> dca
-      (alphabet A)
-      (initial A, 0)
-      (\<lambda> a (p, k). (transition A a p, count (rejecting A) p k))
-      (degen (rejecting A))"
-
-  lemma dgcad_simps[simp]:
-    "dca.alphabet (dgcad A) = alphabet A"
-    "dca.initial (dgcad A) = (initial A, 0)"
-    "dca.transition (dgcad A) a (p, k) = (transition A a p, count (rejecting A) p k)"
-    "dca.rejecting (dgcad A) = degen (rejecting A)"
-    unfolding dgcad_def by auto
-
-  lemma dgcad_target[simp]: "dca.target (dgcad A) w (p, k) =
-    (dgca.target A w p, fold (count (rejecting A)) (butlast (p # dgca.states A w p)) k)"
-    by (induct w arbitrary: p k) (auto)
-  lemma dgcad_states[simp]: "dca.states (dgcad A) w (p, k) =
-    dgca.states A w p || scan (count (rejecting A)) (p # dgca.states A w p) k"
-    by (induct w arbitrary: p k) (auto)
-  lemma dgcad_trace[simp]: "dca.trace (dgcad A) w (p, k) =
-    dgca.trace A w p ||| sscan (count (rejecting A)) (p ## dgca.trace A w p) k"
-    by (coinduction arbitrary: w p k) (auto)
-  lemma dgcad_path[iff]: "dca.path (dgcad A) w (p, k) \<longleftrightarrow> dgca.path A w p"
-    unfolding DCA.path_alt_def DGCA.path_alt_def by simp
-  lemma dgcad_run[iff]: "dca.run (dgcad A) w (p, k) \<longleftrightarrow> dgca.run A w p"
-    unfolding DCA.run_alt_def DGCA.run_alt_def by simp
-
-  (* TODO: revise *)
-  lemma dgcad_nodes_fst[simp]: "fst ` DCA.nodes (dgcad A) = DGCA.nodes A"
-    unfolding dca.nodes_alt_def dca.reachable_alt_def
-    unfolding dgca.nodes_alt_def dgca.reachable_alt_def
-    unfolding image_def by simp
-  lemma dgcad_nodes_snd_empty:
-    assumes "rejecting A = []"
-    shows "snd ` DCA.nodes (dgcad A) \<subseteq> {0}"
-  proof -
-    have 2: "snd (dca.transition (dgcad A) a (p, k)) = 0" for a p k using assms by auto
-    show ?thesis using 2 by (auto elim: dca.nodes.cases)
-  qed
-  lemma dgcad_nodes_snd_nonempty:
-    assumes "rejecting A \<noteq> []"
-    shows "snd ` DCA.nodes (dgcad A) \<subseteq> {0 ..< length (rejecting A)}"
-  proof -
-    have 1: "snd (dca.initial (dgcad A)) < length (rejecting A)"
-      using assms by simp
-    have 2: "snd (dca.transition (dgcad A) a (p, k)) < length (rejecting A)" for a p k
-      using assms by auto
-    show ?thesis using 1 2 by (auto elim: dca.nodes.cases)
-  qed
-  lemma dgcad_nodes_empty:
-    assumes "rejecting A = []"
-    shows "DCA.nodes (dgcad A) = DGCA.nodes A \<times> {0}"
-  proof -
-    have "(p, k) \<in> DCA.nodes (dgcad A) \<longleftrightarrow> p \<in> fst ` DCA.nodes (dgcad A) \<and> k = 0" for p k
-      using dgcad_nodes_snd_empty[OF assms] by (force simp del: dgcad_nodes_fst)
-    then show ?thesis by auto
-  qed
-  lemma dgcad_nodes_nonempty:
-    assumes "rejecting A \<noteq> []"
-    shows "DCA.nodes (dgcad A) \<subseteq> DGCA.nodes A \<times> {0 ..< length (rejecting A)}"
-    using subset_fst_snd dgcad_nodes_fst[of A] dgcad_nodes_snd_nonempty[OF assms] by blast
-  lemma dgcad_nodes: "DCA.nodes (dgcad A) \<subseteq> DGCA.nodes A \<times> {0 ..< max 1 (length (rejecting A))}"
-    using dgcad_nodes_empty dgcad_nodes_nonempty by force
-
-  lemma dgcad_language[simp]: "DCA.language (dgcad A) = DGCA.language A" by force
-
-  lemma dgcad_nodes_finite[iff]: "finite (DCA.nodes (dgcad A)) \<longleftrightarrow> finite (DGCA.nodes A)"
-  proof
-    show "finite (DGCA.nodes A)" if "finite (DCA.nodes (dgcad A))"
-      using that by (auto simp flip: dgcad_nodes_fst)
-    show "finite (DCA.nodes (dgcad A))" if "finite (DGCA.nodes A)"
-      using dgcad_nodes that finite_subset by fastforce
-  qed
-  lemma dgcad_nodes_card: "card (DCA.nodes (dgcad A)) \<le> max 1 (length (rejecting A)) * card (DGCA.nodes A)"
-  proof (cases "finite (DGCA.nodes A)")
-    case True
-    have "card (DCA.nodes (dgcad A)) \<le> card (DGCA.nodes A \<times> {0 ..< max 1 (length (rejecting A))})"
-      using dgcad_nodes True by (blast intro: card_mono)
-    also have "\<dots> = max 1 (length (rejecting A)) * card (DGCA.nodes A)" unfolding card_cartesian_product by simp
-    finally show ?thesis by this
-  next
-    case False
-    then have "card (DGCA.nodes A) = 0" "card (DCA.nodes (dgcad A)) = 0" by auto
-    then show ?thesis by simp
-  qed
+  abbreviation successors where "successors \<equiv> dgca.successors TYPE('label)"
 
 end
