thys/Transition_Systems_and_Automata/Automata/DRA/DRA_Refine.thy
@@ -13,7 +13,7 @@ begin
       (alphabet A\<^sub>1, alphabet A\<^sub>2) \<in> \<langle>L\<rangle> set_rel \<and>
       (initial A\<^sub>1, initial A\<^sub>2) \<in> S \<and>
       (transition A\<^sub>1, transition A\<^sub>2) \<in> L \<rightarrow> S \<rightarrow> S \<and>
-      (accepting A\<^sub>1, accepting A\<^sub>2) \<in> \<langle>rabin_rel S\<rangle> list_rel}"
+      (condition A\<^sub>1, condition A\<^sub>2) \<in> \<langle>rabin_rel S\<rangle> list_rel}"
 
   lemma dra_param[param]:
     "(dra, dra) \<in> \<langle>L\<rangle> set_rel \<rightarrow> S \<rightarrow> (L \<rightarrow> S \<rightarrow> S) \<rightarrow> \<langle>rabin_rel S\<rangle> list_rel \<rightarrow>
@@ -21,7 +21,7 @@ begin
     "(alphabet, alphabet) \<in> \<langle>L, S\<rangle> dra_rel \<rightarrow> \<langle>L\<rangle> set_rel"
     "(initial, initial) \<in> \<langle>L, S\<rangle> dra_rel \<rightarrow> S"
     "(transition, transition) \<in> \<langle>L, S\<rangle> dra_rel \<rightarrow> L \<rightarrow> S \<rightarrow> S"
-    "(accepting, accepting) \<in> \<langle>L, S\<rangle> dra_rel \<rightarrow> \<langle>rabin_rel S\<rangle> list_rel"
+    "(condition, condition) \<in> \<langle>L, S\<rangle> dra_rel \<rightarrow> \<langle>rabin_rel S\<rangle> list_rel"
     unfolding dra_rel_def fun_rel_def by auto
 
   lemma dra_rel_id[simp]: "\<langle>Id, Id\<rangle> dra_rel = Id" unfolding dra_rel_def using dra.expand by auto
@@ -29,11 +29,11 @@ begin
     assumes [param]: "(A, B) \<in> \<langle>L\<^sub>1, S\<^sub>1\<rangle> dra_rel" "(B, C) \<in> \<langle>L\<^sub>2, S\<^sub>2\<rangle> dra_rel"
     shows "(A, C) \<in> \<langle>L\<^sub>1 O L\<^sub>2, S\<^sub>1 O S\<^sub>2\<rangle> dra_rel"
   proof -
-    have "(accepting A, accepting B) \<in> \<langle>rabin_rel S\<^sub>1\<rangle> list_rel" by parametricity
-    also have "(accepting B, accepting C) \<in> \<langle>rabin_rel S\<^sub>2\<rangle> list_rel" by parametricity
-    finally have 1: "(accepting A, accepting C) \<in> \<langle>rabin_rel S\<^sub>1 O rabin_rel S\<^sub>2\<rangle> list_rel" by simp
+    have "(condition A, condition B) \<in> \<langle>rabin_rel S\<^sub>1\<rangle> list_rel" by parametricity
+    also have "(condition B, condition C) \<in> \<langle>rabin_rel S\<^sub>2\<rangle> list_rel" by parametricity
+    finally have 1: "(condition A, condition C) \<in> \<langle>rabin_rel S\<^sub>1 O rabin_rel S\<^sub>2\<rangle> list_rel" by simp
     have 2: "rabin_rel S\<^sub>1 O rabin_rel S\<^sub>2 \<subseteq> rabin_rel (S\<^sub>1 O S\<^sub>2)" by (force simp: fun_rel_def)
-    have 3: "(accepting A, accepting C) \<in> \<langle>rabin_rel (S\<^sub>1 O S\<^sub>2)\<rangle> list_rel" using 1 2 list_rel_mono by blast
+    have 3: "(condition A, condition C) \<in> \<langle>rabin_rel (S\<^sub>1 O S\<^sub>2)\<rangle> list_rel" using 1 2 list_rel_mono by blast
     have "(transition A, transition B) \<in> L\<^sub>1 \<rightarrow> S\<^sub>1 \<rightarrow> S\<^sub>1" by parametricity
     also have "(transition B, transition C) \<in> L\<^sub>2 \<rightarrow> S\<^sub>2 \<rightarrow> S\<^sub>2" by parametricity
     finally have 4: "(transition A, transition C) \<in> L\<^sub>1 O L\<^sub>2 \<rightarrow> S\<^sub>1 O S\<^sub>2 \<rightarrow> S\<^sub>1 O S\<^sub>2" by this
@@ -56,18 +56,18 @@ begin
   lemma dra_rel_eq: "(A, A) \<in> \<langle>Id_on (alphabet A), Id_on (nodes A)\<rangle> dra_rel"
     unfolding dra_rel_def prod_rel_def using list_all2_same[to_set] by auto
 
-  lemma enableds_param[param]: "(enableds, enableds) \<in> \<langle>L, S\<rangle> dra_rel \<rightarrow> S \<rightarrow> \<langle>L\<rangle> set_rel"
-    using dra_param(2, 4) unfolding dra.enableds_def fun_rel_def set_rel_def by fastforce
-  lemma paths_param[param]: "(paths, paths) \<in> \<langle>L, S\<rangle> dra_rel \<rightarrow> S \<rightarrow> \<langle>\<langle>L\<rangle> list_rel\<rangle> set_rel"
-    unfolding paths_def by (intro fun_relI paths_param, fold enableds_def) (parametricity+)
-  lemma runs_param[param]: "(runs, runs) \<in> \<langle>L, S\<rangle> dra_rel \<rightarrow> S \<rightarrow> \<langle>\<langle>L\<rangle> stream_rel\<rangle> set_rel"
-    unfolding runs_def by (intro fun_relI runs_param, fold enableds_def) (parametricity+)
+  lemma enableds_param[param]: "(dra.enableds, dra.enableds) \<in> \<langle>L, S\<rangle> dra_rel \<rightarrow> S \<rightarrow> \<langle>L\<rangle> set_rel"
+    unfolding dra.enableds_def by simp parametricity
+  lemma paths_param[param]: "(dra.paths, dra.paths) \<in> \<langle>L, S\<rangle> dra_rel \<rightarrow> S \<rightarrow> \<langle>\<langle>L\<rangle> list_rel\<rangle> set_rel"
+    using enableds_param[param_fo] by parametricity
+  lemma runs_param[param]: "(dra.runs, dra.runs) \<in> \<langle>L, S\<rangle> dra_rel \<rightarrow> S \<rightarrow> \<langle>\<langle>L\<rangle> stream_rel\<rangle> set_rel"
+    using enableds_param[param_fo] by parametricity
 
   lemma reachable_param[param]: "(reachable, reachable) \<in> \<langle>L, S\<rangle> dra_rel \<rightarrow> S \<rightarrow> \<langle>S\<rangle> set_rel"
   proof -
-    have 1: "reachable A p = (\<lambda> w. target A w p) ` paths A p" for A :: "('label, 'state) dra" and p
+    have 1: "reachable A p = (\<lambda> w. target A w p) ` dra.paths A p" for A :: "('label, 'state) dra" and p
       unfolding dra.reachable_alt_def dra.paths_def by auto
-    show ?thesis unfolding 1 by parametricity
+    show ?thesis unfolding 1 using enableds_param[param_fo] by parametricity
   qed
   lemma nodes_param[param]: "(nodes, nodes) \<in> \<langle>L, S\<rangle> dra_rel \<rightarrow> \<langle>S\<rangle> set_rel"
   proof -
@@ -78,11 +78,11 @@ begin
 
   lemma language_param[param]: "(language, language) \<in> \<langle>L, S\<rangle> dra_rel \<rightarrow> \<langle>\<langle>L\<rangle> stream_rel\<rangle> set_rel"
   proof -
-    have 1: "language A = (\<Union> w \<in> runs A (initial A).
-      if cogen rabin (accepting A) (trace A w (initial A)) then {w} else {})"
+    have 1: "language A = (\<Union> w \<in> dra.runs A (initial A).
+      if cogen rabin (condition A) (trace A w (initial A)) then {w} else {})"
       for A :: "('label, 'state) dra"
-      unfolding language_def dra.runs_def image_def by auto
-    show ?thesis unfolding 1 by parametricity
+      unfolding dra.language_def dra.runs_def by auto
+    show ?thesis unfolding 1 using enableds_param[param_fo] by parametricity
   qed
 
 end
