thys/Transition_Systems_and_Automata/Basic/Basic.thy
@@ -10,6 +10,10 @@ begin
 
   lemmas [simp] = map_prod.id map_prod.comp[symmetric]
   lemma prod_UNIV[iff]: "A \<times> B = UNIV \<longleftrightarrow> A = UNIV \<and> B = UNIV" by auto
+  lemma prod_singleton:
+    "fst ` A = {x} \<Longrightarrow> A = fst ` A \<times> snd ` A"
+    "snd ` A = {y} \<Longrightarrow> A = fst ` A \<times> snd ` A"
+    by force+
 
   lemma infinite_subset[trans]: "infinite A \<Longrightarrow> A \<subseteq> B \<Longrightarrow> infinite B" using infinite_super by this
   lemma finite_subset[trans]: "A \<subseteq> B \<Longrightarrow> finite B \<Longrightarrow> finite A" using finite_subset by this
